specIR/SIRUnstackproof.v
@@ -1,0 +1,614 @@
+From Coq Require Import
+     Arith.PeanoNat
+     Lists.List
+     Strings.String
+     Morphisms
+     Setoid
+     RelationClasses.
+
+Require Import MapsC.
+Require Import ValuesC.
+Require Import MemoryC.
+Require Import CoqlibC.
+Require Import ASTC.
+Require Import EventsC.
+Require Import GlobalenvsC.
+Require Import IntegersC.
+Require Import Mod ModSem Any Skeleton.
+Require Import SimMem SimSymb Sound.
+Require SimMemId SimSymbId SoundTop.
+Require Import SimMod SimModSem.
+Require Import SIRCommon SIRStack CtypesC ClightC.
+
+Require Import Program.
+Require Import Simulation.
+
+Set Implicit Arguments.
+
+
+
+Definition Kbot := Kstop.
+
+Inductive kle: cont -> cont -> Prop :=
+(* | kle_refl *)
+(*     k *)
+(*   : *)
+(*     kle k k *)
+| kle_bot
+    k
+  :
+    kle Kbot k
+| Kseq_le
+    st
+    k0 k1
+    (LE: kle k0 k1)
+  :
+    kle (Kseq st k0) (Kseq st k1)
+| Kloop1_le
+    cond body
+    k0 k1
+    (LE: kle k0 k1)
+  :
+    kle (Kloop1 cond body k0) (Kloop1 cond body k1)
+| Kloop2_le
+    cond body
+    k0 k1
+    (LE: kle k0 k1)
+  :
+    kle (Kloop2 cond body k0) (Kloop2 cond body k1)
+| Kswitch_le
+    k0 k1
+    (LE: kle k0 k1)
+  :
+    kle (Kswitch k0) (Kswitch k1)
+| Kcall_le
+    oid fd e te
+    k0 k1
+    (LE: kle k0 k1)
+  :
+    kle (Kcall oid fd e te k0) (Kcall oid fd e te k1)
+.
+
+Program Instance kle_Reflexive: Reflexive kle.
+Next Obligation.
+  induction x; ii; ss; try (by econs; et).
+Qed.
+
+Lemma kle_refl k: kle k k. Proof. refl. Qed.
+Hint Resolve kle_refl.
+
+Inductive state_le: state -> state -> Prop :=
+| State_le
+    fd st e le m
+    k0 k1
+    (LE: kle k0 k1)
+  :
+    state_le (State fd st k0 e le m) (State fd st k1 e le m)
+| Callstate_le
+    fptr ty vs m
+    k0 k1
+    (LE: kle k0 k1)
+  :
+    state_le (Callstate fptr ty vs k0 m) (Callstate fptr ty vs k1 m)
+| Returnstate_le
+    v m k0 k1
+    (LE: kle k0 k1)
+  :
+    state_le (Returnstate v k0 m) (Returnstate v k1 m)
+.
+
+Lemma kle_call_cont
+      k0 k1
+      (LE: kle k0 k1)
+  :
+    kle (call_cont k0) (call_cont k1)
+.
+Proof.
+  ginduction k0; ii; ss; try inv LE; try econs; et; ss; et.
+Qed.
+
+(* Lemma kle_find_label: forall *)
+(*       lbl body res *)
+(*       k0 k1 *)
+(*       (KLE: kle k0 k1) *)
+(*       (LBL: find_label lbl body k0 = Some res) *)
+(*   , *)
+(*     <<LBL: find_label lbl body k1 = Some res>> *)
+(* with *)
+(* kle_find_label_ls: forall *)
+(*     lbl body res *)
+(*     k0 k1 *)
+(*     (KLE: kle k0 k1) *)
+(*     (LBL: find_label_ls lbl body k0 = Some res) *)
+(*   , *)
+(*     <<LBL: find_label_ls lbl body k1 = Some res>> *)
+(* . *)
+(* Proof. *)
+(*   - ii. destruct body; ss. *)
+(*     + des_ifs; et. *)
+(*       * *)
+(*   - ii. move body at top. revert_until kle_find_label_ls. induction body; ii; ss. *)
+(*     + destruct body1; ss; et. *)
+(*       * destruct body1; ss. eapply kle_find_label. *)
+(* Qed. *)
+
+Lemma step_step
+      se ge st_bot0 tr st_bot1 st0
+      (NOGOTO: True)
+      (STEP: step2 se ge st_bot0 tr st_bot1)
+      (LE: state_le st_bot0 st0)
+  :
+    exists st1, <<STEP: step2 se ge st0 tr st1>> /\ <<LE: state_le st_bot1 st1>>
+.
+Proof.
+  inv STEP; inv LE; try inv LE0; ss; try (by esplits; repeat (econs; ss; eauto using kle_call_cont)).
+  - esplits; et.
+    + econs; ss; et. TTTTTTTTTTTTTTTTTTT <--------- this does not hold. Kbot is not really bot.
+  - admit "goto".
+  - admit "goto".
+  - admit "goto".
+  - admit "goto".
+Qed.
+
+Lemma plus_plus
+      se ge st_bot0 tr st_bot1 st0
+      (NOGOTO: True)
+      (STEP: plus step2 se ge st_bot0 tr st_bot1)
+      (LE: state_le st_bot0 st0)
+  :
+    exists st1, <<STEP: plus step2 se ge st0 tr st1>> /\ <<LE: state_le st_bot1 st1>>
+.
+Proof.
+  admit "ez".
+Admitted.
+
+
+
+Section OWNEDHEAP.
+
+Variable mi: string.
+Variable md_src: SMod.t unit.
+Variable p_tgt: program.
+Let p_src := SMod.prog md_src.
+Let md_tgt := module2_mi p_tgt (Some mi).
+Hypothesis (MISRC: md_src.(SMod.midx) = mi).
+Variable skenv_link: SkEnv.t.
+Let ms_src := md_src skenv_link.
+Let ms_tgt := md_tgt skenv_link.
+
+Let skenv: SkEnv.t := (SkEnv.project skenv_link) (CSk.of_program signature_of_function p_tgt).
+Let ge: genv := Build_genv (SkEnv.revive (skenv) p_tgt) p_tgt.(prog_comp_env).
+
+Notation ktr :=
+  (ktree (eff1 unit) (unit * (mem * val)) (unit * (mem * val)))
+.
+Notation itr := (itree (eff1 unit) (unit * (mem * val))).
+
+
+
+(*** sim syntax ***)
+Section SYNTAX.
+
+(*** sim itree ***)
+Let fr_src := itree (E unit) (unit * (mem * val)).
+Let fr_tgt := Clight.state.
+
+Section FRAME.
+
+Inductive _match_fr (match_fr: fr_src -> fr_tgt -> Prop): fr_src -> fr_tgt -> Prop :=
+| match_fr_ret
+    oh0 m0 v0
+  :
+    _match_fr match_fr (Ret (oh0, (m0, v0))) (Returnstate v0 Kbot m0)
+| match_fr_tau
+    st_src0 st_tgt0 st_tgt1
+    (SIM: match_fr st_src0 st_tgt1)
+    (TGT: Plus ms_tgt st_tgt0 E0 st_tgt1)
+  :
+    _match_fr match_fr (tau;; st_src0) (st_tgt0)
+| match_fr_icall
+    fname oh0 m0 vs0
+    fblk ty fd
+    (SYMB: Genv.find_symbol ge fname = Some fblk)
+    (FINDF: Genv.find_funct ge (Vptr fblk Ptrofs.zero) = Some (Ctypes.Internal fd))
+    (TY: type_of_fundef (Ctypes.Internal fd) = ty)
+
+    k_src
+    (* (SIM: match_fr st_src0 st_tgt0) *)
+    (* (TGT: Plus ms_tgt st_tgt0 E0 st_tgt1) *)
+  :
+    _match_fr match_fr
+              (Vis (subevent _ (ICall fname oh0 m0 vs0)) k_src)
+              (Callstate (Vptr fblk Ptrofs.zero) ty vs0 Kbot m0)
+| match_fr_ub
+    kt st0
+  :
+    _match_fr match_fr
+              (Vis (subevent _ (EUB)) kt)
+              st0
+| match_fr_ecall
+    fptr oh0 m0 vs0 k_src
+    sg targs tres cconv
+    (EXTERNAL: Genv.find_funct ge fptr = None)
+    (SG: (signature_of_type targs tres cconv) = sg)
+    (SIG: exists skd, (Genv.find_funct skenv_link) fptr = Some skd
+                      /\ Some (signature_of_type targs tres cconv) = Sk.get_csig skd)
+  :
+    _match_fr match_fr
+              (Vis (subevent _ (ECall sg fptr oh0 m0 vs0)) k_src)
+              (Callstate fptr (Tfunction targs tres cconv) vs0 Kbot m0)
+.
+
+Definition match_fr: _ -> _ -> Prop := paco2 _match_fr bot2.
+Lemma match_fr_mon: monotone2 _match_fr.
+Proof.
+  ii. destruct IN; try (by econs; et; rr; et).
+Qed.
+
+End FRAME.
+Hint Unfold match_fr.
+Hint Resolve match_fr_mon: paco.
+
+
+
+
+
+
+(*** I don't use record style in order not to contaminate namespace ***)
+(* Inductive stack: Type := *)
+(* | mk_stack *)
+(*     (optid: option ident) *)
+(*     (fd: Clight.function) *)
+(*     (e: env) *)
+(*     (le: temp_env) *)
+(* . *)
+
+(***
+[ktr] [ktr] [tau ;; Ret 10]
+let k0 := Kcall _ _ Kbot in
+let k1 := Kcall _ _ k1 in
+Callstate k1
+***)
+
+Inductive match_stack: list ktr -> cont -> Prop :=
+| match_stack_nil
+  :
+    match_stack [] Kstop
+| match_stack_cons
+    hd tl
+    oid fd e te ktl
+    (TL: match_stack tl ktl)
+    (HD: forall oh0 m0 r0,
+        match_fr (hd (oh0, (m0, r0)))
+                 (State fd Sskip ktl e (set_opttemp oid r0 te) m0))
+  :
+    match_stack (hd :: tl) (Kcall oid fd e te ktl)
+.
+
+Inductive match_states: SIRStack.state unit -> state -> Prop :=
+| match_states_intro
+    cur_src cont_src
+    fptr ty vs ktl m0
+    (CUR: match_fr cur_src (Callstate fptr ty vs Kbot m0))
+    (CONT: match_stack cont_src ktl)
+  :
+    match_states (mk cur_src cont_src) (Callstate fptr ty vs ktl m0)
+.
+
+Inductive match_func: SIRCommon.function unit -> function -> Prop :=
+| match_func_intro
+    kt fd
+    (SIM: forall
+        oh0 m0 vs0
+        e le m1
+        (ENTRY: function_entry2 ge fd vs0 m0 e le m1)
+      ,
+        match_fr (kt oh0 m0 vs0) (State fd fd.(fn_body) Kbot e le m1))
+  :
+    match_func kt fd
+
+.
+
+Inductive match_prog: (SIRCommon.program unit) -> program -> Prop :=
+| match_prog_intro
+    p_src p_tgt
+    (PROG: forall
+        id
+        (SRC: is_some (p_src id))
+      ,
+        <<TGT: is_some ((prog_defmap (program_of_program p_tgt)) ! id)>>)
+    (SIM: forall
+        id f_src f_tgt
+        (SRC: p_src id = Some f_src)
+        (TGT: ((prog_defmap (program_of_program p_tgt)) ! id) = Some (Gfun (Internal f_tgt)))
+      ,
+        <<SIM: match_func f_src f_tgt>>)
+  :
+    match_prog p_src p_tgt
+.
+
+(* Inductive match_states: SIRStack.state unit -> state -> Prop := *)
+(* (* | match_states_nil *) *)
+(* (*     oh0 m0 v0 *) *)
+(* (*   : *) *)
+(* (*     match_states (Ret (oh0, (m0, v0))) (Returnstate v0 Kbot m0) *) *)
+(* | match_states_start *)
+(*   : *)
+(*     match_states (it0) (Callstate fptr ty vs0 k0 m0) *)
+(* . *)
+
+(* Inductive match_stack (stk_src: ktr) (stk_tgt: stack): Prop := *)
+(* | match_stack_intro *)
+(*     optid fd e le *)
+(*     (TGT: stk_tgt = mk_stack optid fd e le) *)
+(*     (SIM: forall oh0 m0 v0, *)
+(*         match_states (stk_src (oh0, (m0, v0))) *)
+(*                      (State fd Clight.Sskip Kunused e (set_opttemp optid v0 le) m0)) *)
+(* . *)
+
+End SYNTAX.
+Hint Unfold match_fr.
+Hint Constructors match_prog match_func match_states match_stack.
+Hint Resolve match_fr_mon: paco.
+
+
+
+Let SMO := SimMemOh_default_aux _ (Some mi).
+Local Existing Instance SMO.
+
+Tactic Notation "substs" :=
+  repeat (match goal with H: ?x = ?y |- _ =>
+            first [ subst x | subst y ] end).
+
+Ltac inv H := inversion H; clear H; substs.
+
+Lemma match_states_lxsim
+      st_src0 st_tgt0 smo0
+      (MATCH: match_states st_src0 st_tgt0)
+  :
+    <<XSIM: lxsim ms_src ms_tgt 
+                  (fun _ => () -> exists (_ : ()) (_ : mem), True)
+                  (Ord.lift_idx unit_ord_wf tt) st_src0 st_tgt0 smo0>>
+.
+Proof.
+  revert_until SMO.
+  pcofix CIH. i. pfold.
+  ii. clear SUSTAR.
+  inv MATCH.
+  punfold CUR. inv CUR.
+  - pclearbot.
+    + ss. econs 1. ii. econs 1; swap 2 3.
+      { split; intro T; rr in T; des; ss; inv T; ss. }
+      { eapply modsem_receptive; et. }
+      ii. inv STEPSRC; ss. clarify. substs.
+      exploit plus_plus; et.
+      { instantiate (1:= Callstate fptr ty vs ktl m0). econs; et. econs; et.
+      esplits; et.
+      * left. eapply ModSemProps.spread_dplus.
+        { eapply modsem2_mi_determinate; et. }
+        ss; et.
+      * right. eapply CIH. econs; ss; et.
+Qed.
+
+
+
+
+
+
+
+
+Section SIM.
+
+  Hypothesis (SIMP: match_prog p_src p_tgt).
+
+  Lemma match_prog_sim_st
+        i_src i_tgt
+        (SIM: match_itr i_src i_tgt)
+    :
+      sim_st bot2 tt (interp_mrec (interp_function p_src) i_src)
+             (interp_mrec (interp_function p_tgt) i_tgt)
+  .
+  Proof.
+    revert_until SIMP.
+    ginit.
+    { intros. eapply cpn3_wcompat; et. eauto with paco. }
+    gcofix CIH.
+    i. rewrite ! unfold_interp_mrec.
+    punfold SIM. inv SIM; cbn.
+    - gstep. econs; et.
+    - pclearbot. gstep. econs; et. gbase. et.
+    - pclearbot. gstep. econs; et. gbase.
+      eapply CIH. eapply match_itr_bind.
+      { u. ii. repeat spc MATCH. pclearbot. eauto. }
+      exploit (@SIMP fname); et. intro T. r in T. des_ifs; cycle 1.
+      { pfold. econs; et. }
+      exploit T; et.
+    - gstep. econs; et. u in *. gstep. econs; et. repeat spc MATCH. specialize (MATCH H0).
+      des; ss. gbase. eapply CIH.
+      eauto with paco.
+    - gstep. econs; et.
+    - gstep. econs; et.
+    - gstep. econs; et. ii. exploit SIM0; et. i; des_safe. pclearbot. esplits.
+      gstep. econs; et. eauto with paco.
+    - gstep. des. pclearbot. econs; et. esplits; et. gstep.
+      rewrite (unfold_interp_mrec _ (Tau i_tgt0)). cbn. econs; et. eauto with paco.
+    - gstep. pclearbot. econs; et. ii. repeat spc SIM0. gstep.
+      rewrite (unfold_interp_mrec _ (Tau i_src0)). cbn. econs; et. eauto with paco.
+  Unshelve.
+    all: ss.
+  Qed.
+
+  (*** The result that we wanted -- allows reasoning each function "locally" and then compose ***)
+  Theorem adequacy_local_local:
+    forall
+      (fname: ident) m vs oh_src oh_tgt
+      (O: SO oh_src oh_tgt)
+    ,
+      (<<SIM: sim_st bot2 tt (interp_program p_src (ICall fname oh_src m vs))
+                     (interp_program p_tgt (ICall fname oh_tgt m vs))
+                     >>)
+  .
+  Proof.
+    {
+      ii.
+      eapply match_prog_sim_st; ss.
+      hexploit (@SIMP fname); et. intro T. r in T. des_ifs; cycle 1.
+      { pfold. econs; et. }
+      repeat (spc T). des. ss.
+    }
+  Qed.
+
+  Hypothesis (SIMMI: mi_src = mi_tgt).
+  Hypothesis (SIMO: forall skenv, SO (md_src.(SMod.initial_owned_heap) skenv)
+                                     (md_tgt.(SMod.initial_owned_heap) skenv)).
+  Hypothesis (SIMSK: md_src.(SMod.sk) = md_tgt.(SMod.sk)).
+  Let mp: ModPair.t := (SimSymbId.mk_mp md_src md_tgt).
+
+  Theorem sim_mod: ModPair.sim mp.
+  Proof.
+    eapply SimSIR.sim_mod; eauto.
+    econs; et.
+    { eapply unit_ord_wf. }
+    ii. clarify. esplits. eapply adequacy_local_local; et.
+  Qed.
+
+  Theorem correct: rusc defaultR [md_src: Mod.t] [md_tgt: Mod.t].
+  Proof. eapply AdequacyLocal.relate_single_rusc; try exists mp; esplits; eauto using sim_mod. Qed.
+
+  Lemma match_itr_bind_assume
+        P x y
+        (MATCH: match_itr x y)
+    :
+      <<MATCH: match_itr (assume P ;; x) (assume P ;; y)>>
+  .
+  Proof.
+    Fail eapply match_itr_bind.
+    Fail progress f_equiv.
+    (*** Like in SIRHoare, we need to parameterize "match_itr" in order to do this.
+         However, we can't do that for arbitrary type S. (because it is not leibniz equality)
+         TODO: current design is somewhat unsatisfactory. Probably what we want is following:
+           - SIRLocalStrong: src/tgt can have different value/mem/owned_heap,
+                             but weak match_itr_bind
+           - SIRLocalWeak: src/tgt should have (leibniz) equal value/mem/owned_heap,
+                           but strong match_itr_bind
+     ***)
+    unfold assume. des_ifs; irw; ss.
+    unfold triggerUB. irw. pfold; econs; et.
+  Qed.
+
+  Lemma match_itr_bind_guarantee
+        P x y
+        (MATCH: match_itr x y)
+    :
+      <<MATCH: match_itr (guarantee P ;; x) (guarantee P ;; y)>>
+  .
+  Proof.
+    unfold guarantee. des_ifs; irw; ss.
+    unfold triggerNB. irw. pfold; econs; et.
+  Qed.
+
+End SIM.
+
+End OWNEDHEAP.
+Hint Unfold match_itr match_fn match_prog.
+Hint Resolve match_itr_mon: paco.
+Hint Constructors bindC: core.
+
+
+Section REFL.
+  Variable owned_heap: Type.
+  Global Program Instance match_itr_Reflexive: Reflexive (match_itr (@eq owned_heap)).
+  Next Obligation.
+    rr. revert x.
+    ginit.
+    { intros. eapply cpn2_wcompat; eauto with paco. }
+    gcofix CIH. ii. gstep.
+    ides x.
+    - destruct r0 as [oh [m vs]]. econs; et.
+    - econs; et. eauto with paco.
+    - destruct e.
+      + destruct i. econs; et. ii. rr in H. des_ifs. des; clarify. eauto with paco.
+      + destruct s.
+        * destruct e. econs; et. ii. rr in H. des_ifs. des; clarify. eauto with paco.
+        * destruct e; try econs; et. ii. esplits; et. eauto with paco.
+  Qed.
+  
+  Global Program Instance match_fn_Reflexive: Reflexive (match_fn (@eq owned_heap)).
+  Next Obligation.
+    ii. clarify. r. refl.
+  Qed.
+
+  Global Program Instance match_prog_Reflexive: Reflexive (match_prog (@eq owned_heap)).
+  Next Obligation.
+    ii. clarify. r. des_ifs. r. refl.
+  Qed.
+
+End REFL.
+
+
+
+(*** TODO: move to CoqlibC ***)
+Ltac unfoldr term :=
+  first[
+      unfold term at 10|
+      unfold term at 9|
+      unfold term at 8|
+      unfold term at 7|
+      unfold term at 6|
+      unfold term at 5|
+      unfold term at 4|
+      unfold term at 3|
+      unfold term at 2|
+      unfold term at 1|
+      unfold term at 0
+    ]
+.
+
+Ltac step :=
+  match goal with
+  | [ |- SIRLocal.match_itr eq (assume _ ;; _) (assume _ ;; _) ] =>
+    eapply match_itr_bind_assume; irw
+  | [ |- SIRLocal.match_itr eq (guarantee _ ;; _) (guarantee _ ;; _) ] =>
+    eapply match_itr_bind_guarantee; irw
+  | [ |- SIRLocal.match_itr eq (assume ?P ;; _) _ ] =>
+    unfoldr assume;
+    let name := fresh "_ASSUME" in
+    destruct (ClassicalDescription.excluded_middle_informative P) as [name|name]; cycle 1; [
+      unfold triggerUB;
+      rewrite bind_vis (*** <---------- this is counter-intuitive. Any good idea? ***);
+      pfold; by (econs; eauto)|irw]
+  | [ |- SIRLocal.match_itr eq (guarantee ?P ;; _) _ ] =>
+    unfoldr guarantee;
+    let name := fresh "_GUARANTEE" in
+    destruct (ClassicalDescription.excluded_middle_informative P) as [name|name]; cycle 1; [
+      contradict name|irw]
+  | [ |- SIRLocal.match_itr eq ((match ?x with _ => _ end) >>= guaranteeK _)
+                            (match ?y with _ => _ end) ] =>
+    tryif (check_equal x y)
+    then let name := fresh "_DES" in
+         destruct x eqn:name; clarify; irw
+    else fail
+  | [ |- SIRLocal.match_itr eq (triggerUB >>= _) _ ] =>
+    unfold triggerUB; irw;
+    pfold; by (econs; eauto)
+  | [ |- SIRLocal.match_itr eq _ (triggerNB >>= _) ] =>
+    unfold triggerNB; irw;
+    pfold; by (econs; eauto)
+  | [ |- SIRLocal.match_itr eq (guaranteeK ?P ?x) _ ] =>
+    unfold guaranteeK;
+    let name := fresh "_GUARANTEEK" in
+    destruct (ClassicalDescription.excluded_middle_informative (P x)) as [name|name]; cycle 1; [
+      contradict name|irw]
+  | [ |- SIRLocal.match_itr eq (Ret _) (Ret _) ] =>
+    pfold; try (by econs; eauto)
+  | [ |- SIRLocal.match_itr eq (Vis (subevent _ (ICall _ _ _ _)) _)
+                            (Vis (subevent _ (ICall _ _ _ _)) _) ] =>
+    pfold; eapply match_icall; ss; et
+  | [ |- HProper _ _ _ ] => ii
+  | [ H: SALL _ _ _ |- _ ] => r in H; des_ifs_safe; des; clarify
+  | [ |- upaco2 (_match_itr ?SO) bot2 _ _ ] =>
+    left;
+    replace (paco2 (_match_itr SO) bot2) with (SIRLocal.match_itr SO) by ss;
+    irw
+  end
+.
